Run bootstrap compilation with cv_compute

cv_translator/eval_cake_compileLib.sml
@@ -1,0 +1,122 @@
+(*
+  Functions for in-logic evaluation of the CakeML compiler.
+  These use HOL's cv_compute facility.
+*)
+structure eval_cake_compileLib :> eval_cake_compileLib =
+struct
+
+open preamble cv_transLib;
+open exportTheory;
+open to_data_cvTheory;
+
+type arch_thms =
+  { default_config_def : thm
+  , to_livesets_def    : thm
+  , compile_cake_def   : thm
+  , cv_export_def      : thm }
+
+type comp_input =
+  { prefix               : string
+  , conf_def             : thm
+  , prog_def             : thm
+  , output_filename      : string
+  , output_conf_filename : string option }
+
+fun write_cv_char_list_to_file filename cv_char_list_tm = let
+  val f = TextIO.openOut filename
+  fun loop tm = let
+    val (n,rest) = cvSyntax.dest_cv_pair tm
+    val c = cvSyntax.dest_cv_num n |> numSyntax.int_of_term |> chr
+    val _ = TextIO.output1(f,c)
+    in loop rest end handle HOL_ERR _ => ();
+  val _ = loop cv_char_list_tm
+  in TextIO.closeOut f end;
+
+fun eval_cake_compile_general (arch : arch_thms) (input : comp_input) = let
+  val { prefix, conf_def, prog_def
+      , output_filename , output_conf_filename } = input
+  val { default_config_def, to_livesets_def
+      , compile_cake_def, cv_export_def } = arch
+  fun define_abbrev name tm =
+    Feedback.trace ("Theory.allow_rebinds", 1)
+      (mk_abbrev (prefix ^ name)) tm
+  val conf = conf_def |> concl |> lhs
+  val c = backendTheory.config_to_inc_config_def
+            |> ISPEC conf |> CONV_RULE (RAND_CONV EVAL)
+  val _ = cv_trans_deep_embedding EVAL prog_def
+  val input_tm = to_livesets_def |> GEN_ALL
+    |> SPEC (prog_def |> concl |> lhs)
+    |> SPEC (c |> concl |> rand) |> concl |> lhs |> mk_fst
+  val oracles = let
+    val graphs = cv_eval input_tm |> rconc
+    in reg_allocComputeLib.get_oracle reg_alloc.Irc graphs end
+  val oracle_def = define_abbrev "oracle" oracles;
+  val _ = cv_trans_deep_embedding EVAL oracle_def
+  val oracle_tm = oracle_def |> concl |> lhs
+  val c_tm = c |> concl |> lhs
+  val c_oracle_tm = backend_cvTheory.inc_set_oracle_def
+                      |> SPEC (c |> concl |> rhs)
+                      |> SPEC oracle_tm |> concl |> lhs
+  val input_tm = compile_cake_def |> GEN_ALL
+    |> SPEC (prog_def |> concl |> lhs)
+    |> SPEC c_oracle_tm |> concl |> lhs
+  val to_option_some = cv_typeTheory.to_option_def |> cj 2
+  val to_pair = cv_typeTheory.to_pair_def |> cj 1
+  val th1 = cv_eval_raw input_tm
+            |> CONV_RULE (PATH_CONV "lr" (REWRITE_CONV [GSYM c]))
+  val th2 = th1 |> CONV_RULE (PATH_CONV "r" (REWR_CONV to_option_some))
+            handle HOL_ERR _ => failwith "compiler returned NONE"
+  val th3 = th2 |> CONV_RULE (PATH_CONV "rr" (REWR_CONV to_pair))
+                |> CONV_RULE (PATH_CONV "rrr" (REWR_CONV to_pair))
+                |> CONV_RULE (PATH_CONV "rrrr" (REWR_CONV to_pair))
+                |> CONV_RULE (PATH_CONV "rrrrr" (REWR_CONV to_pair))
+  fun abbrev_inside name path th = let
+    val tm = dest_path path (concl th)
+    val def = define_abbrev name tm
+    in (def, CONV_RULE (PATH_CONV path (REWR_CONV (SYM def))) th) end
+  val (code_def,th) = abbrev_inside "code" "rrlr" th3
+  val (data_def,th) = abbrev_inside "data" "rrrlr" th
+  val (ffis_def,th) = abbrev_inside "ffis" "rrrrlr" th
+  val (syms_def,th) = abbrev_inside "syms" "rrrrrlr" th
+  val (conf_def,th) = abbrev_inside "conf" "rrrrrr" th
+  val result_th = th
+  (* --- *)
+  val e = cv_export_def |> concl |> strip_forall |> snd |> lhs
+  val cv_ty = cvSyntax.cv
+  fun get_one_subst name abbrev_def =
+    mk_var(name,cvSyntax.cv) |-> (abbrev_def |> concl |> rhs |> rand)
+  fun cv_explode e = SPEC e basis_cvTheory.cv_mlstring_explode_def |> concl |> lhs
+  fun cv_concat e = SPEC e basis_cvTheory.cv_mlstring_concat_def |> concl |> lhs
+  fun cv_append e = SPEC e basis_cvTheory.cv_misc_append_def |> concl |> lhs
+  val export_tm = e |> cv_append |> cv_concat |> cv_explode |> subst
+    [get_one_subst "cv_ffi_names" ffis_def,
+     get_one_subst "cv_data" data_def,
+     get_one_subst "cv_bytes" code_def,
+     get_one_subst "cv_syms" syms_def]
+  val _ = null (free_vars export_tm) orelse failwith "failed to eval export"
+  (*
+    cv_repLib.cv_rep_for []
+    “explode $ concat $ misc$append (x64_export x64_ffis x64_code x64_data x64_syms)”
+  *)
+  val l = cv_computeLib.cv_compute (cv_transLib.cv_eqs_for export_tm) export_tm
+          |> concl |> rhs
+  val _ = write_cv_char_list_to_file output_filename l
+  val _ = case output_conf_filename of NONE => ()
+          | SOME fname => write_cv_char_list_to_file fname
+                            (conf_def |> concl |> rhs |> rand)
+  in th end
+
+fun eval_cake_compile_with_conf arch prefix conf_def prog_def filename =
+  eval_cake_compile_general arch
+    { prefix               = prefix
+    , conf_def             = conf_def
+    , prog_def             = prog_def
+    , output_filename      = filename
+    , output_conf_filename = NONE };
+
+fun eval_cake_compile arch prefix =
+  eval_cake_compile_with_conf arch prefix (#default_config_def arch);
+
+val _ = Feedback.set_trace "TheoryPP.include_docs" 0;
+
+end
