cv_translator/backend_x64_evalScript.sml
@@ -1,97 +1,16 @@
 (*
   Experiments with evaluating the compiler using cv_compute
 *)
-open preamble cv_transLib;
-open backend_x64_cvTheory x64_configTheory;
-open exportTheory export_x64Theory;
-open to_data_cvTheory;
+open preamble;
 
 val _ = new_theory "backend_x64_eval";
 
-fun write_cv_char_list_to_file filename cv_char_list_tm = let
-  val f = TextIO.openOut filename
-  fun loop tm = let
-    val (n,rest) = cvSyntax.dest_cv_pair tm
-    val c = cvSyntax.dest_cv_num n |> numSyntax.int_of_term |> chr
-    val _ = TextIO.output1(f,c)
-    in loop rest end handle HOL_ERR _ => ();
-  val _ = loop cv_char_list_tm
-  in TextIO.closeOut f end;
+open eval_cake_compile_x64Lib;
 
-fun compile_cake prefix conf prog filename conf_filename = let
-  fun define_abbrev name tm =
-    Feedback.trace ("Theory.allow_rebinds", 1)
-      (mk_abbrev (prefix ^ name)) tm
-  val c = backendTheory.config_to_inc_config_def
-            |> ISPEC conf |> CONV_RULE (RAND_CONV EVAL)
-  val input_tm = backend_x64Theory.to_livesets_x64_def |> GEN_ALL
-    |> SPEC prog |> SPEC (c |> concl |> rand) |> concl |> lhs |> mk_fst
-  val oracles = let
-    val graphs = cv_eval input_tm |> rconc
-    in reg_allocComputeLib.get_oracle reg_alloc.Irc graphs end
-  val oracle_def = define_abbrev "oracle" oracles;
-  val _ = cv_trans_deep_embedding EVAL oracle_def
-  val oracle_tm = oracle_def |> concl |> lhs
-  val c_tm = c |> concl |> lhs
-  val c_oracle_tm = backend_cvTheory.inc_set_oracle_def
-                      |> SPEC (c |> concl |> rhs)
-                      |> SPEC oracle_tm |> concl |> lhs
-  val input_tm = backend_x64Theory.compile_cake_x64_def |> GEN_ALL
-    |> SPEC prog |> SPEC c_oracle_tm |> concl |> lhs
-  val to_option_some = cv_typeTheory.to_option_def |> cj 2
-  val to_pair = cv_typeTheory.to_pair_def |> cj 1
-  val th1 = cv_eval_raw input_tm
-            |> CONV_RULE (PATH_CONV "lr" (REWRITE_CONV [GSYM c]))
-  val th2 = th1 |> CONV_RULE (PATH_CONV "r" (REWR_CONV to_option_some))
-            handle HOL_ERR _ => failwith "compiler returned NONE"
-  val th3 = th2 |> CONV_RULE (PATH_CONV "rr" (REWR_CONV to_pair))
-                |> CONV_RULE (PATH_CONV "rrr" (REWR_CONV to_pair))
-                |> CONV_RULE (PATH_CONV "rrrr" (REWR_CONV to_pair))
-                |> CONV_RULE (PATH_CONV "rrrrr" (REWR_CONV to_pair))
-  fun abbrev_inside name path th = let
-    val tm = dest_path path (concl th)
-    val def = define_abbrev name tm
-    in (def, CONV_RULE (PATH_CONV path (REWR_CONV (SYM def))) th) end
-  val (code_def,th) = abbrev_inside "code" "rrlr" th3
-  val (data_def,th) = abbrev_inside "data" "rrrlr" th
-  val (ffis_def,th) = abbrev_inside "ffis" "rrrrlr" th
-  val (syms_def,th) = abbrev_inside "syms" "rrrrrlr" th
-  val (conf_def,th) = abbrev_inside "conf" "rrrrrr" th
-  val result_th = th
-  (* --- *)
-  val e = cv_x64_export_def |> concl |> strip_forall |> snd |> lhs
-  val cv_ty = cvSyntax.cv
-  fun get_one_subst name abbrev_def =
-    mk_var(name,cvSyntax.cv) |-> (abbrev_def |> concl |> rhs |> rand)
-  fun cv_explode e = SPEC e cv_mlstring_explode_def |> concl |> lhs
-  fun cv_concat e = SPEC e cv_mlstring_concat_def |> concl |> lhs
-  fun cv_append e = SPEC e cv_misc_append_def |> concl |> lhs
-  val export_tm = e |> cv_append |> cv_concat |> cv_explode |> subst
-    [get_one_subst "cv_ffi_names" ffis_def,
-     get_one_subst "cv_data" data_def,
-     get_one_subst "cv_bytes" code_def,
-     get_one_subst "cv_syms" syms_def]
-  val _ = null (free_vars export_tm) orelse failwith "failed to eval export"
-  (*
-    cv_repLib.cv_rep_for []
-    “explode $ concat $ misc$append (x64_export x64_ffis x64_code x64_data x64_syms)”
-  *)
-  val l = cv_computeLib.cv_compute (cv_transLib.cv_eqs_for export_tm) export_tm
-          |> concl |> rhs
-  val _ = write_cv_char_list_to_file filename l
-  val _ = case conf_filename of NONE => ()
-          | SOME fname => write_cv_char_list_to_file fname
-                            (conf_def |> concl |> rhs |> rand)
-  in th end
+Definition prog_def:
+  prog = [] : ast$dec list
+End
 
-(*
-val _ = (max_print_depth := 15);
-val prefix = "x64_"
-val conf = “x64_backend_config”
-val prog = “[] : ast$dec list”
-val filename = "output.S"
-val conf_filename = SOME "conf_str.txt"
-val res = time (compile_cake prefix conf prog filename) conf_filename;
-*)
+val res = eval_cake_compile_x64 "" prog_def "empty_prog.S";
 
 val _ = export_theory();
