compiler/bootstrap/compilation/x64/64/alt_x64BootstrapScript.sml
@@ -1,0 +1,11 @@
+(*
+  Evaluateof the 64-bit version of the compiler into x64 machine code.
+*)
+open preamble compiler64ProgTheory eval_cake_compile_x64Lib;
+
+val _ = new_theory "alt_x64Bootstrap"
+
+Theorem compiler64_compiled =
+  eval_cake_compile_x64 "" compiler64_prog_def "cake.S";
+
+val _ = export_theory ();
